# Copyright (c) 2022 Orange. All rights reserved.
#
# Redistribution and use in source and binary forms, with or without modification, are permitted provided that the following conditions are met:
#     1. Redistributions of source code must retain the above copyright notice, this list of conditions and the following disclaimer.
#     2. Redistributions in binary form must reproduce the above copyright notice, this list of conditions and the following disclaimer in the documentation and/or other materials provided with the distribution.
#     3. All advertising materials mentioning features or use of this software must display the following acknowledgement:
#     This product includes software developed by Orange.
#     4. Neither the name of Orange nor the names of its contributors may be used to endorse or promote products derived from this software without specific prior written permission.
#
# THIS SOFTWARE IS PROVIDED BY Orange "AS IS" AND ANY EXPRESS OR IMPLIED WARRANTIES, INCLUDING, BUT NOT LIMITED TO, THE IMPLIED WARRANTIES OF MERCHANTABILITY AND FITNESS FOR A PARTICULAR PURPOSE ARE DISCLAIMED. IN NO EVENT SHALL Orange BE LIABLE FOR ANY DIRECT, INDIRECT, INCIDENTAL, SPECIAL, EXEMPLARY, OR CONSEQUENTIAL DAMAGES (INCLUDING, BUT NOT LIMITED TO, PROCUREMENT OF SUBSTITUTE GOODS OR SERVICES; LOSS OF USE, DATA, OR PROFITS; OR BUSINESS INTERRUPTION) HOWEVER CAUSED AND ON ANY THEORY OF LIABILITY, WHETHER IN CONTRACT, STRICT LIABILITY, OR TORT (INCLUDING NEGLIGENCE OR OTHERWISE) ARISING IN ANY WAY OUT OF THE USE OF THIS SOFTWARE, EVEN IF ADVISED OF THE POSSIBILITY OF SUCH DAMAGE.

@prefix rdf: <http://www.w3.org/1999/02/22-rdf-syntax-ns#> .
@prefix owl: <http://www.w3.org/2002/07/owl#> .
@prefix skos: <http://www.w3.org/2004/02/skos/core#> .
@prefix rdfs: <http://www.w3.org/2000/01/rdf-schema#> .
@prefix xsd: <http://www.w3.org/2001/XMLSchema#> .

@prefix foaf: <http://xmlns.com/foaf/0.1/> .
@prefix dc: <http://purl.org/dc/elements/1.1/> .
@prefix dcterms: <http://purl.org/dc/terms/> .

@prefix voc: <https://w3id.org/noria/kos/> .

voc:oss
    a skos:ConceptScheme;
    skos:definition "Operation Support System (OSS).";
    skos:notation "oss" ;
	# --- Vocab metadata ---
	dcterms:issued "2022-05-10"^^xsd:date ;
	dcterms:publisher <https://www.orange.com/> ;
	dcterms:creator <https://orcid.org/0000-0001-5887-899X> ;  # Lionel Tailhardat
	dcterms:creator <https://orcid.org/0000-0001-5639-1504> ;  # Yoan Chabot
	dcterms:creator <https://orcid.org/0000-0003-0457-1436> ;  # Raphaël Troncy
	dcterms:license <https://spdx.org/licenses/BSD-4-Clause> ;
    dcterms:title "The NORIA Operation Support System (OSS) vocabulary." ;
    dcterms:type <https://nkos.dublincore.org/#thesaurus> ;
.

# =============================================================================

<https://w3id.org/noria/kos/oss/process>
    a skos:ConceptScheme;
    skos:definition "Recommended process in relation to OSSs (Operation Support Systems).";
    skos:inScheme voc:oss ;
    skos:notation "process" .

<https://w3id.org/noria/kos/oss/process/change-management>
    a skos:Concept;
    skos:definition "Change management.";
    skos:inScheme <https://w3id.org/noria/kos/oss/process>;
    skos:notation "change-management";
    skos:prefLabel "Change Management Process"@en .

<https://w3id.org/noria/kos/oss/process/incident-management>
    a skos:Concept;
    skos:definition """Incident management: an incident is a failure or a deterioration of service detected and declared by the customer or by internal operator.
    The associated process is to find and solve the causes of the incident and to restore the service.
    The incident is an urgent situation calling for a very short term action and resolution"""@en;
    skos:inScheme <https://w3id.org/noria/kos/oss/process>;
    skos:related <https://w3id.org/noria/kos/oss/process/problem-management>;
    skos:notation "incident-management";
    skos:prefLabel "Incident Management Process"@en .

<https://w3id.org/noria/kos/oss/process/problem-management>
    a skos:Concept;
    skos:definition """Problem management: a problem is a risky situation which can cause an incident and is generally observed by internal operators.
    The associated process is to analyse the causes of the problem and to correct them in order to avoid the incident from occurring.
    The problem is a middle / long term situation calling for deep analysis and reliable solution."""@en;
    skos:inScheme <https://w3id.org/noria/kos/oss/process>;
    skos:related <https://w3id.org/noria/kos/oss/process/incident-management>;
    skos:notation "problem-management";
    skos:prefLabel "Problem Management Process"@en .

<https://w3id.org/noria/kos/oss/process/anomaly-report>
    a skos:Concept;
    skos:definition "Anomaly report.";
    skos:inScheme <https://w3id.org/noria/kos/oss/process>;
    skos:notation "anomaly-report";
    skos:prefLabel "Anomaly Report"@en .

# -----------------------------------------------------------------------------

<https://w3id.org/noria/kos/oss/gnoc-roles>
    a skos:ConceptScheme;
    skos:definition "Users roles involved in GNOC (Global Network Operation Center) processes (i.e. incident management and change management).";
    skos:inScheme voc:oss ;
    skos:notation "gnoc-roles" .

<https://w3id.org/noria/kos/oss/gnoc-roles/icr>
    a skos:Concept;
    skos:definition """Responsible for coordination of failure removal, i.e. to restore service in the shortest possible time and to minimize failure impact.
    All high priority incidents (e.g. Priority 1 and 2) are managed by the ICR."""@en;
    skos:inScheme <https://w3id.org/noria/kos/oss/gnoc-roles>;
    skos:notation "icr";
    skos:prefLabel "Incident Coordinator"@en .

<https://w3id.org/noria/kos/oss/gnoc-roles/ccr>
    a skos:Concept;
    skos:definition """Responsible for coordination of all changes realized by the GNOC.
    Identifies/prevents risks in changes (e.g. situations when changes each with no impact, could generate incidents if performed simultaneously).
    All changes with high impact/risk are managed by the CCR."""@en;
    skos:inScheme <https://w3id.org/noria/kos/oss/gnoc-roles>;
    skos:notation "ccr";
    skos:prefLabel "Change Coordinator"@en .

<https://w3id.org/noria/kos/oss/gnoc-roles/tir>
    a skos:Concept;
    skos:definition "Entity or person identifying the incident and opening the trouble ticket.";
    skos:inScheme <https://w3id.org/noria/kos/oss/gnoc-roles>;
    skos:notation "tir";
    skos:prefLabel "Ticket Initiator"@en .

<https://w3id.org/noria/kos/oss/gnoc-roles/mcc>
    a skos:Concept;
    skos:definition "Entity or person to be contacted for feedback or escalation.";
    skos:inScheme <https://w3id.org/noria/kos/oss/gnoc-roles>;
    skos:notation "mcc";
    skos:prefLabel "Main Customer Contact"@en .

# -----------------------------------------------------------------------------

<https://w3id.org/noria/kos/oss/technical-objects>
    a skos:ConceptScheme;
    skos:definition """High-level objects, managed by OSS components, which represent the elements of Orange and the customers’ networks and services."""@en;
    skos:inScheme voc:oss ;
    skos:notation "technical-objects" .

<https://w3id.org/noria/kos/oss/technical-objects/product>
    a skos:Concept;
    skos:definition """A Product is a service provided and charged to the customer and it relies on one or several Resources.
    A Product is associated to a customer and it can carry warranties and SLAs.
    These two points make the difference between Resource and Product."""@en;
    skos:inScheme <https://w3id.org/noria/kos/oss/technical-objects>;
    skos:notation "product";
    skos:prefLabel "Product"@en .

<https://w3id.org/noria/kos/oss/technical-objects/resource>
    a skos:Concept;
    skos:definition """The Resources are shared elements of the network on which the Customers' Products and Services are implemented."""@en;
    skos:inScheme <https://w3id.org/noria/kos/oss/technical-objects>;
    skos:notation "resource";
    skos:prefLabel "Resource"@en .

<https://w3id.org/noria/kos/oss/technical-objects/non-managed-product>
    a skos:Concept;
    skos:definition "Object necessary to describe a technical component to carry operations and where there is no record of the technical element."@en;
    skos:inScheme <https://w3id.org/noria/kos/oss/technical-objects>;
    skos:notation "non-managed-product";
    skos:prefLabel "Non-managed Product"@en .
